ffi/ByteStringFFI.v
@@ -1,0 +1,49 @@
+(** This is the code we intend to approximate with the FFI refined version of
+    ByteString:
+
+  import Data.Word8
+  import GHC.ForeignPtr
+  import GHC.IO
+
+  data ByteString = PS {-# UNPACK #-} !(ForeignPtr Word8) -- payload
+                       {-# UNPACK #-} !Int                -- offset
+                       {-# UNPACK #-} !Int                -- length
+      deriving (Typeable)
+
+  {--[ cons ]---------------------------------------------------------------}
+
+  mallocByteString :: Int -> IO (ForeignPtr a)
+  mallocByteString l = GHC.mallocPlainForeignPtrBytes l
+
+  create :: Int -> (Ptr Word8 -> IO ()) -> IO ByteString
+  create l f = do
+      fp <- mallocByteString l
+      withForeignPtr fp $ \p -> f p
+      return $! PS fp 0 l
+
+  unsafeCreate :: Int -> (Ptr Word8 -> IO ()) -> ByteString
+  unsafeCreate l f = unsafeDupablePerformIO (create l f)
+
+  foreign import ccall unsafe "string.h memcpy" c_memcpy
+      :: Ptr Word8 -> Ptr Word8 -> CSize -> IO (Ptr Word8)
+
+  memcpy :: Ptr Word8 -> Ptr Word8 -> Int -> IO ()
+  memcpy p q s = c_memcpy p q (fromIntegral s) >> return ()
+
+  cons :: Word8 -> ByteString -> ByteString
+  cons c (PS x s l) = unsafeCreate (l+1) $ \p -> withForeignPtr x $ \f -> do
+          poke p c
+          memcpy (p `plusPtr` 1) (f `plusPtr` s) (fromIntegral l)
+
+  {--[ uncons ]-------------------------------------------------------------}
+
+  accursedUnutterablePerformIO :: IO a -> a
+  accursedUnutterablePerformIO (IO m) = case m realWorld# of (# _, r #) -> r
+
+  uncons :: ByteString -> Maybe (Word8, ByteString)
+  uncons (PS x s l)
+      | l <= 0    = Nothing
+      | otherwise = Just (accursedUnutterablePerformIO $ withForeignPtr x
+                                                       $ \p -> peekByteOff p s,
+                          PS x (s+1) (l-1))
+*)
