ffi/HeapFFI.v
@@ -1,0 +1,265 @@
+Require Import
+  ByteString.Lib.Tactics
+  ByteString.Lib.Nomega
+  ByteString.Lib.Fiat
+  ByteString.Lib.FromADT
+  ByteString.Lib.TupleEnsembles
+  ByteString.Lib.FunMaps
+  ByteString.Memory
+  ByteString.Heap
+  ByteString.HeapState
+  ByteString.ByteString
+  ByteString.ByteStringHeap
+  Coq.FSets.FMapFacts
+  Coq.Structures.DecidableTypeEx.
+
+Module HeapFFI (M : WSfun N_as_DT).
+
+Module Import Heap := Heap M.
+
+Import HeapState.
+Import FMapExt.
+
+Module Import FunMaps := FunMaps N_as_DT M.
+
+Open Scope N_scope.
+
+Record Mem (Env : Type) := {
+  heap_ptr : Env;
+  heap_rep : EMap Ptr Size;
+  mem_rep  : EMap Ptr Word;
+}.
+
+Definition Mem_AbsR (Env : Type) (or : Rep HeapSpec) (nr : Mem Env) :=
+  Map_AbsR eq (heap_rep nr) (resvs or) /\
+  Map_AbsR eq (mem_rep nr)  (bytes or).
+
+Record HeapIntf (Env : Type) := {
+  nullPtr      : Ptr;
+  alignPtr     : Ptr -> Size -> Ptr;
+  plusPtr      : Ptr -> Size -> Ptr;
+  minusPtr     : Ptr -> Size -> Ptr;
+
+  mallocBytes  : Size -> Mem Env -> (Ptr * Mem Env);
+  freeBytes    : Ptr -> Mem Env -> Mem Env;
+  reallocBytes : Ptr -> Size -> Mem Env -> (Ptr * Mem Env);
+
+  peekPtr      : Ptr -> Mem Env -> (Word * Mem Env);
+  peekByteOff  : Ptr -> Size -> Mem Env -> (Word * Mem Env);
+  pokePtr      : Ptr -> Word -> Mem Env -> Mem Env;
+  pokeByteOff  : Ptr -> Size -> Word -> Mem Env -> Mem Env;
+
+  copyBytes    : Ptr -> Ptr -> Size -> Mem Env -> Mem Env;
+  fillBytes    : Ptr -> Word -> Size -> Mem Env -> Mem Env;
+
+  newheap_relates : forall mem, @Mem_AbsR Env newHeapState mem;
+
+  malloc_relates : forall env env' sz ptr,
+    mallocBytes (` sz) env = (ptr, env')
+      -> forall r r', alloc r sz ↝ (r', ptr)
+      -> Mem_AbsR r' env';
+
+  malloc_sound : forall env env' sz ptr,
+    mallocBytes sz env = (ptr, env') ->
+      All (fun ptr' sz' => ~ overlaps ptr' sz' ptr sz) (heap_rep env);
+
+  free_relates : forall env env' ptr,
+    freeBytes ptr env = env'
+      -> forall r r', free r ptr ↝ (r', tt)
+      -> Mem_AbsR r' env';
+
+  realloc_relates : forall env env' old sz new,
+    reallocBytes old (` sz) env = (new, env')
+      -> forall r r', realloc r old sz ↝ (r', new)
+      -> Mem_AbsR r' env';
+
+  realloc_sound : forall env env' sz old new,
+    reallocBytes old sz env = (new, env') ->
+      All (fun ptr' sz' => ~ overlaps ptr' sz' new sz)
+          (Remove old (heap_rep env));
+
+  peek_relates : forall env env' ptr w,
+    peekPtr ptr env = (w, env')
+      -> forall r r', peek r ptr ↝ (r', w)
+      -> Mem_AbsR r' env';
+
+  peek_sound : forall env env' ptr w,
+    Lookup ptr w (mem_rep env) -> peekPtr ptr env = (w, env');
+
+  poke_relates : forall env env' ptr w,
+    pokePtr ptr w env = env'
+      -> forall r r', poke r ptr w ↝ (r', tt)
+      -> Mem_AbsR r' env';
+
+  memcpy_relates : forall env env' addr1 addr2 sz,
+    copyBytes addr1 sz addr2 env = env'
+      -> forall r r', memcpy r addr1 addr2 sz ↝ (r', tt)
+      -> Mem_AbsR r' env';
+
+  memset_relates : forall env env' addr w sz,
+    fillBytes addr w sz env = env'
+      -> forall r r', memset r addr sz w ↝ (r', tt)
+      -> Mem_AbsR r' env'
+}.
+
+(** In order to refine to a computable heap, we have to add the notion of
+    "free memory", from which addresses may be allocated. A further
+    optimization here would be to add a free list, to which free blocks are
+    returned, in order avoid gaps in the heap. A yet further optimization
+    would be to better manage the free space to avoid fragmentation. The
+    implementation below simply grows the heap with every allocation. *)
+
+Theorem HeapFFI {Env : Type} (ffi : HeapIntf Env) (mem : Mem Env) :
+  FullySharpened HeapSpec.
+Proof.
+  intros.
+  start sharpening ADT.
+
+  hone representation over HeapSpec using (@Mem_AbsR Env).
+
+  (* refine method emptyS. *)
+  {
+    rewrite refine_pick.
+      instantiate (1 := ret mem).
+      finish honing.
+
+    intros.
+    apply newheap_relates; assumption.
+  }
+
+  (* refine method allocS. *)
+  {
+    unfold find_free_block.
+    refine pick val (fst (mallocBytes ffi (` d) r_n)).
+    {
+      remember (mallocBytes _ _ _) as malloc.
+      simplify with monad laws; simpl.
+
+      refine pick val (snd malloc).
+        simplify with monad laws; simpl.
+        rewrite Heqmalloc.
+        finish honing.
+
+      symmetry in Heqmalloc.
+      destruct malloc as [addr env'].
+
+      eapply malloc_relates; eauto.
+      repeat econstructor; apply PickComputes.
+
+      destruct H0.
+      pose proof (malloc_sound _ _ Heqmalloc) as H2.
+      eapply All_Map_AbsR in H2; relational; eauto.
+      constructor; split; nomega_.
+    }
+
+    remember (mallocBytes _ _ _) as malloc.
+    symmetry in Heqmalloc.
+    destruct malloc as [addr env'].
+
+    destruct H0.
+    pose proof (malloc_sound _ _ Heqmalloc) as H2.
+    eapply All_Map_AbsR in H2; relational; eauto.
+    constructor; split; nomega_.
+  }
+
+  (* refine method freeS. *)
+  {
+    refine pick val (freeBytes ffi d r_n).
+      simplify with monad laws; simpl.
+      finish honing.
+
+    eapply free_relates; auto.
+    repeat econstructor.
+  }
+
+  (* refine method reallocS. *)
+  {
+    unfold find_free_block.
+    refine pick val (fst (reallocBytes ffi d (` d0) r_n)).
+    {
+      remember (reallocBytes _ _ _ _) as realloc.
+      simplify with monad laws.
+
+      refine pick val (snd realloc).
+        simplify with monad laws.
+        rewrite Heqrealloc.
+        finish honing.
+
+      symmetry in Heqrealloc.
+      destruct realloc as [addr env'].
+
+      eapply realloc_relates; eauto.
+      repeat econstructor; apply PickComputes.
+
+      destruct H0.
+      pose proof (realloc_sound _ _ Heqrealloc) as H2.
+      eapply All_Map_AbsR in H2; relational; eauto;
+      related_maps; eauto.
+      constructor; split; nomega_.
+    }
+
+    remember (reallocBytes _ _ _ _) as realloc.
+    symmetry in Heqrealloc.
+    destruct realloc as [addr env'].
+
+    destruct H0.
+    pose proof (realloc_sound _ _ Heqrealloc) as H2.
+    eapply All_Map_AbsR in H2; relational; eauto;
+    related_maps; eauto.
+    constructor; split; nomega_.
+  }
+
+  (* refine method peekS. *)
+  {
+    refine pick val (fst (peekPtr ffi d r_n)).
+      simplify with monad laws.
+      refine pick val r_n.
+        simplify with monad laws.
+        finish honing.
+      assumption.
+
+    intros.
+    apply H0 in H1; destruct H1 as [? [? ?]]; subst.
+    eapply (peek_sound ffi r_n r_n d) in H1; eauto.
+    rewrite H1.
+    reflexivity.
+  }
+
+  (* refine method pokeS. *)
+  {
+    refine pick val (pokePtr ffi d d0 r_n).
+      simplify with monad laws.
+      finish honing.
+
+    eapply poke_relates; eauto.
+    repeat econstructor.
+  }
+
+  (* refine method memcpyS. *)
+  {
+    refine pick val (copyBytes ffi d d1 d0 r_n).
+      simplify with monad laws.
+      finish honing.
+
+    eapply memcpy_relates; eauto.
+    repeat econstructor.
+  }
+
+  (* refine method memsetS. *)
+  {
+    refine pick val (fillBytes ffi d d1 d0 r_n).
+      simplify with monad laws.
+      finish honing.
+
+    eapply memset_relates; eauto.
+    repeat econstructor.
+  }
+
+  finish_SharpeningADT_WithoutDelegation.
+Defined.
+
+Definition HeapFFI' {Env : Type} (ffi : HeapIntf Env) (mem : Mem Env) :=
+  Eval simpl in projT1 (HeapFFI ffi mem).
+Print HeapFFI'.
+
+End HeapFFI.
